Properties.v
@@ -1814,8 +1814,8 @@ Proof.
   auto.
 Qed.
 
-Lemma WfMod_Hidden m:
-  WfMod m ->
+Lemma WfMod_Hidden ty m:
+  WfMod ty m ->
   forall s, In s (getHidden m) -> In s (map fst (getAllMethods m)).
 Proof.
   induction 1; simpl; auto; intros.
@@ -2012,8 +2012,8 @@ Lemma flatten_Substeps m o l:
   - econstructor 3; eauto.
 Qed.
 
-Lemma Step_substitute' m o l:
-  Step m o l -> forall (HWfMod: WfMod m), StepSubstitute m o l.
+Lemma Step_substitute' ty m o l:
+  Step m o l -> forall (HWfMod: WfMod ty m), StepSubstitute m o l.
 Proof.
   unfold StepSubstitute.
   induction 1; auto; simpl; intros; dest; unfold MatchingExecCalls_Base in *; simpl in *.
@@ -2084,7 +2084,7 @@ Proof.
         destruct (HMatching1 _ n H7); contradiction.
 Qed.
 
-Lemma StepSubstitute_flatten m o l (HWfMod: WfMod m):
+Lemma StepSubstitute_flatten ty m o l (HWfMod: WfMod ty m):
   Step (flatten m) o l <-> StepSubstitute m o l.
 Proof.
   unfold flatten, getFlat, StepSubstitute.
@@ -2108,12 +2108,12 @@ Proof.
       rewrite createHide_Meths; auto.
 Qed.
     
-Lemma Step_substitute m o l (HWfMod: WfMod m):
+Lemma Step_substitute ty m o l (HWfMod: WfMod ty m):
   Step m o l -> Step (flatten m) o l.
 Proof.
   intros Stp.
-  apply Step_substitute' in Stp; auto.
-  rewrite StepSubstitute_flatten in *; auto.
+  apply (@Step_substitute' ty) in Stp; auto.
+  rewrite (@StepSubstitute_flatten ty) in *; auto.
 Qed.
 
 Definition concatFlat m1 m2 := BaseMod (getRegisters m1 ++ getRegisters m2)
@@ -2570,8 +2570,8 @@ Section SplitSubsteps.
   Variable DisjRules: DisjKey (getRules m1) (getRules m2).
   Variable DisjMeths: DisjKey (getMethods m1) (getMethods m2).
 
-  Variable WfMod1: WfBaseMod m1.
-  Variable WfMod2: WfBaseMod m2.
+  Variable WfMod1: forall ty, WfBaseMod ty m1.
+  Variable WfMod2: forall ty, WfBaseMod ty m2.
   
   Lemma filter_perm o l :
     Substeps (concatFlat m1 m2) o l ->
@@ -2651,7 +2651,8 @@ Section SplitSubsteps.
       destruct HInRules as [HInRules|HInRules];generalize (in_map fst _ _ HInRules);destruct DisjRules;try contradiction.
       + subst; dest; exists x, x0;split;[|split;[|split;[|split]]];auto.
         rewrite (InRules_Filter _ _ _ _ _ _ HInRules).
-        destruct WfMod1 as [WfMod_Rle1 WfMod_Meth1];destruct WfMod2 as [WfMod_Rle2 WfMod_Meth2]; specialize (WfActionT_ReadsWellDefined (WfMod_Rle1 _ HInRules) HAction) as Reads_sublist; specialize (WfActionT_WritesWellDefined (WfMod_Rle1 _ HInRules) HAction) as Writes_sublist.
+        destruct (WfMod1 type) as [WfMod_Rle1 WfMod_Meth1];destruct (WfMod2 type) as [WfMod_Rle2 WfMod_Meth2].
+        specialize (WfActionT_ReadsWellDefined (WfMod_Rle1 _ HInRules) HAction) as Reads_sublist; specialize (WfActionT_WritesWellDefined (WfMod_Rle1 _ HInRules) HAction) as Writes_sublist.
         constructor 2 with (rn:= rn)(rb:=rb)(reads:=reads)(u:=u)(cs:=cs)(ls:=(ModuleFilterLabels m1 ls)); auto.
         * specialize (app_sublist_l _ _ H6) as SL_o_x.
           specialize (WfMod_Rle1 (rn, rb) HInRules); specialize (WfActionT_SemAction WfMod_Rle1 H2 HAction SL_o_x H4).
@@ -2666,7 +2667,7 @@ Section SplitSubsteps.
       + subst; dest; exists x, x0; split;[|split;[|split;[|split]]];auto.
         rewrite (NotInRules_Filter _ _ _ _ _ H3); assumption.
         rewrite (InRules_Filter _ _ _ _ _ _ HInRules).
-        destruct WfMod1 as [WfMod_Rle1 WfMod_Meth1];destruct WfMod2 as [WfMod_Rle2 WfMod_Meth2]; specialize (WfActionT_ReadsWellDefined (WfMod_Rle2 _ HInRules) HAction) as Reads_sublist; specialize (WfActionT_WritesWellDefined (WfMod_Rle2 _ HInRules) HAction) as Writes_sublist.
+        destruct (WfMod1 type) as [WfMod_Rle1 WfMod_Meth1];destruct (WfMod2 type) as [WfMod_Rle2 WfMod_Meth2]; specialize (WfActionT_ReadsWellDefined (WfMod_Rle2 _ HInRules) HAction) as Reads_sublist; specialize (WfActionT_WritesWellDefined (WfMod_Rle2 _ HInRules) HAction) as Writes_sublist.
         constructor 2 with (rn:= rn)(rb:=rb)(reads:=reads)(u:=u)(cs:=cs)(ls:=(ModuleFilterLabels m2 ls)); auto.
         * specialize (app_sublist_r _ _ H6) as SL_o_x.
           specialize (WfMod_Rle2 (rn, rb) HInRules); specialize (WfActionT_SemAction WfMod_Rle2 H2 HAction SL_o_x H5).
@@ -2682,7 +2683,7 @@ Section SplitSubsteps.
       destruct HInMeths as [HInMeths|HInMeths];generalize (in_map fst _ _ HInMeths);destruct DisjMeths;try contradiction;intros.
       + subst; dest; exists x, x0;split;[|split;[|split;[|split]]];auto.
         * rewrite (InMethods_Filter _ _ _ _ _ _ _ _ HInMeths).
-          destruct WfMod1 as [WfMod_Rle1 WfMod_Meth1];destruct WfMod2 as [WfMod_Rle2 WfMod_Meth2]; specialize (WfActionT_ReadsWellDefined (WfMod_Meth1 (fn, fb) HInMeths argV) HAction) as Reads_sublist; specialize (WfActionT_WritesWellDefined (WfMod_Meth1 (fn, fb) HInMeths argV) HAction) as Writes_sublist.
+          destruct (WfMod1 type) as [WfMod_Rle1 WfMod_Meth1];destruct (WfMod2 type) as [WfMod_Rle2 WfMod_Meth2]; specialize (WfActionT_ReadsWellDefined (WfMod_Meth1 (fn, fb) HInMeths argV) HAction) as Reads_sublist; specialize (WfActionT_WritesWellDefined (WfMod_Meth1 (fn, fb) HInMeths argV) HAction) as Writes_sublist.
           constructor 3 with (fn:=fn)(fb:=fb)(reads:=reads)(u:=u)(cs:=cs)(argV:=argV)(retV:=retV)(ls:=(ModuleFilterLabels m1 ls)); auto.
           -- specialize (app_sublist_l _ _ H7) as SL_o_x.
              specialize (WfMod_Meth1 (fn, fb) HInMeths argV); specialize (WfActionT_SemAction WfMod_Meth1 H2 HAction SL_o_x H5).
@@ -2694,7 +2695,7 @@ Section SplitSubsteps.
       + subst; dest; exists x, x0;split;[|split;[|split;[|split]]]; auto.
         * rewrite (NotInMethods_Filter _ _ _ _ _ _ _ _ H3); assumption.
         * rewrite (InMethods_Filter _ _ _ _ _ _ _ _ HInMeths).
-          destruct WfMod1 as [WfMod_Rle1 WfMod_Meth1];destruct WfMod2 as [WfMod_Rle2 WfMod_Meth2]; specialize (WfActionT_ReadsWellDefined (WfMod_Meth2 (fn, fb) HInMeths argV) HAction) as Reads_sublist; specialize (WfActionT_WritesWellDefined (WfMod_Meth2 (fn, fb) HInMeths argV) HAction) as Writes_sublist.
+          destruct (WfMod1 type) as [WfMod_Rle1 WfMod_Meth1];destruct (WfMod2 type) as [WfMod_Rle2 WfMod_Meth2]; specialize (WfActionT_ReadsWellDefined (WfMod_Meth2 (fn, fb) HInMeths argV) HAction) as Reads_sublist; specialize (WfActionT_WritesWellDefined (WfMod_Meth2 (fn, fb) HInMeths argV) HAction) as Writes_sublist.
           constructor 3 with (fn:=fn)(fb:=fb)(reads:=reads)(u:=u)(cs:=cs)(argV:=argV)(retV:=retV)(ls:=(ModuleFilterLabels m2 ls)); auto.
           -- specialize (app_sublist_r _ _ H7) as SL_o_x.
              specialize (WfMod_Meth2 (fn, fb) HInMeths argV); specialize (WfActionT_SemAction WfMod_Meth2 H2 HAction SL_o_x H6).
@@ -2835,11 +2836,12 @@ Lemma WeakEqualitySym : forall l1 l2, WeakEquality l1 l2 -> WeakEquality l2 l1.
   firstorder.
 Qed.
 
-Lemma WfNoDups m (HWfMod : WfMod m) :
+Lemma WfNoDups m (HWfMod : forall ty, WfMod ty m) :
     NoDup (map fst (getAllRegisters m)) /\
     NoDup (map fst (getAllMethods m))   /\
     NoDup (map fst (getAllRules m)).
 Proof.
+  specialize (HWfMod (fun _ => unit)).
   induction m.
   - split;[|split];inversion HWfMod; assumption.
   - inversion HWfMod; subst; apply IHm in HWf.
@@ -2886,9 +2888,11 @@ Proof.
         -- inversion_clear ND_Rles1; assumption.
 Qed.
 
-Lemma WfMod_WfBaseMod_flat m (HWfMod : WfMod m):
-  WfBaseMod (getFlat m).
+Lemma WfMod_WfBaseMod_flat m (HWfMod : forall ty, WfMod ty m):
+  forall ty, WfBaseMod ty (getFlat m).
 Proof.
+  intros ty.
+  specialize (HWfMod ty).
   unfold getFlat;induction m.
   - simpl; inversion HWfMod; subst; destruct WfBaseModule.
     unfold WfBaseMod in *; split; intros.
@@ -2947,36 +2951,40 @@ Proof.
 Qed.
 
 Lemma WfConcats : forall (m1 m2 : Mod) (o : RegsT)(l : list FullLabel),
-    WfConcat m2 m1 ->
+    (forall ty, WfConcat ty m2 m1) ->
     Substeps (getFlat m2) o l ->
     (forall (s: string)(v : {x : Kind*Kind & SignT x}), In s (getHidden m1) -> (getNumCalls (s, v) l = 0%Z)).
 Proof.
   intros.
   induction H0; subst.
   - reflexivity.
-  - inversion H; simpl in HInRules;specialize (H2 _ HInRules).
+  - specialize (H type).
+    inversion H; simpl in HInRules;specialize (H2 _ HInRules).
     rewrite getNumCalls_cons; rewrite IHSubsteps;simpl.
     assert (In (fst (s, v)) (getHidden m1)) as P1;auto.
     rewrite (getNumFromCalls_notIn _ _ (WfConcatNotInCalls _ H2 HAction P1)); ring.
-  - inversion H; simpl in HInMeths;specialize (H3 _ HInMeths argV).
+  - specialize (H type).
+    inversion H; simpl in HInMeths;specialize (H3 _ HInMeths argV).
     rewrite getNumCalls_cons; rewrite IHSubsteps;simpl.
     assert (In (fst (s, v)) (getHidden m1)) as P1;auto.
     rewrite (getNumFromCalls_notIn _ _ (WfConcatNotInCalls _ H3 HAction P1)); ring.
 Qed.
 
 Lemma WfConcats_Substeps : forall (m1 : Mod) m2 (o : RegsT)(l : list FullLabel),
-    WfConcat (Base m2) m1 ->
+    (forall ty, WfConcat ty (Base m2) m1) ->
     Substeps m2 o l ->
     forall f, In (fst f) (getHidden m1) -> (getNumCalls f l = 0%Z).
 Proof.
   intros.
   induction H0; subst.
   - reflexivity.
-  - inversion H; simpl in HInRules;specialize (H2 _ HInRules).
+  - specialize (H type).
+    inversion H; simpl in HInRules;specialize (H2 _ HInRules).
     rewrite getNumCalls_cons; rewrite IHSubsteps;simpl.
     assert (In (fst f) (getHidden m1)) as P1;auto.
     rewrite (getNumFromCalls_notIn _ _ (WfConcatNotInCalls _ H2 HAction P1)); ring.
-  - inversion H; simpl in HInMeths;specialize (H3 _ HInMeths argV).
+  - specialize (H type).
+    inversion H; simpl in HInMeths;specialize (H3 _ HInMeths argV).
     rewrite getNumCalls_cons; rewrite IHSubsteps;simpl.
     assert (In (fst f) (getHidden m1)) as P1;auto.
     rewrite (getNumFromCalls_notIn _ _ (WfConcatNotInCalls _ H3 HAction P1)); ring.
@@ -2985,7 +2993,7 @@ Qed.
 
 
 Lemma WfConcats_Step : forall (m1 m2 : Mod) (o : RegsT) (l : list FullLabel),
-    WfConcat m2 m1 ->
+    (forall ty, WfConcat ty m2 m1) ->
     Step m2 o l ->
     (forall f, In (fst f) (getHidden m1) -> (getNumCalls f l = 0%Z)).
 Proof.
@@ -2996,13 +3004,15 @@ Proof.
     specialize (IHStep H); auto.
   - unfold WfConcat in *; simpl in *.
     setoid_rewrite in_app_iff in H.
-    assert (sth1: (forall rule : RuleT, In rule (getAllRules m0) -> WfConcatActionT (snd rule type) m1) /\
-                  (forall meth : string * {x : Signature & MethodT x},
-                      In meth (getAllMethods m0) -> forall v : type (fst (projT1 (snd meth))), WfConcatActionT (projT2 (snd meth) type v) m1)) by
+    assert (sth1: forall ty,
+               (forall rule : RuleT, In rule (getAllRules m0) -> WfConcatActionT (snd rule ty) m1) /\
+               (forall meth : string * {x : Signature & MethodT x},
+                   In meth (getAllMethods m0) -> forall v : ty (fst (projT1 (snd meth))), WfConcatActionT (projT2 (snd meth) ty v) m1)) by
         (firstorder fail).
-    assert (sth2: (forall rule : RuleT, In rule (getAllRules m2) -> WfConcatActionT (snd rule type) m1) /\
-                  (forall meth : string * {x : Signature & MethodT x},
-                      In meth (getAllMethods m2) -> forall v : type (fst (projT1 (snd meth))), WfConcatActionT (projT2 (snd meth) type v) m1) ) by
+    assert (sth2: forall ty,
+               (forall rule : RuleT, In rule (getAllRules m2) -> WfConcatActionT (snd rule ty) m1) /\
+               (forall meth : string * {x : Signature & MethodT x},
+                   In meth (getAllMethods m2) -> forall v : ty (fst (projT1 (snd meth))), WfConcatActionT (projT2 (snd meth) ty v) m1) ) by
         (firstorder fail).
     specialize (IHStep1 sth1).
     specialize (IHStep2 sth2).
@@ -3011,7 +3021,7 @@ Qed.
 
 Lemma WfConcats_Trace : forall (m1 m2 : Mod) (o : RegsT) ls (l : list FullLabel),
     Trace m2 o ls ->
-    WfConcat m2 m1 ->
+    (forall ty, WfConcat ty m2 m1) ->
     forall i,
       nth_error ls i = Some l ->
       (forall f, In (fst f) (getHidden m1) -> (getNumCalls f l = 0%Z)).
@@ -3025,7 +3035,7 @@ Proof.
 Qed.
     
 
-Lemma substitute_Step' m (HWfMod: WfMod m):
+Lemma substitute_Step' m (HWfMod: forall ty, WfMod ty m):
   forall o l,
     StepSubstitute m o l ->
     exists l', Permutation l l' /\
@@ -3035,19 +3045,26 @@ Proof.
   induction m; simpl in *; intros; dest.
   - exists l; split;[apply Permutation_refl|constructor; auto].
     eapply Substeps_flatten; eauto.
-  - inv HWfMod.
-    assert (exists l' : list FullLabel, l [=] l' /\ Step m o l');[apply IHm;auto|dest;exists x;split;auto].
-    constructor 2; auto.
-    intros.
-    unfold getListFullLabel_diff in *;rewrite <-H2.
-    apply H1; auto.
-  - inv HWfMod.
+  - assert (exists l' : list FullLabel, l [=] l' /\ Step m o l');[apply IHm;auto|dest;exists x;split;auto].
+    + intros;
+        specialize (HWfMod ty);
+        inv HWfMod; auto.
+    + constructor 2; auto.
+      intros.
+      unfold getListFullLabel_diff in *;rewrite <-H2.
+      apply H1; auto.
+  - assert (HWf1: forall ty, WfMod ty m1) by (intros; specialize (HWfMod ty); inv HWfMod; auto).
+    assert (HWf2: forall ty, WfMod ty m2) by (intros; specialize (HWfMod ty); inv HWfMod; auto).
     specialize (IHm1 HWf1).
     specialize (IHm2 HWf2).
     destruct (WfNoDups HWf1) as [ND_Regs1 [ND_Meths1 ND_Rules1]].
     destruct (WfNoDups HWf2) as [ND_Regs2 [ND_Meths2 ND_Rules2]].
     specialize (WfMod_WfBaseMod_flat HWf1) as WfBaseMod1.
     specialize (WfMod_WfBaseMod_flat HWf2) as WfBaseMod2.
+    pose proof (HWfMod (fun _ => unit)) as hwfmod2.
+    assert (WfConcat1: forall ty, WfConcat ty m1 m2 ) by (intros; specialize (HWfMod ty); inv HWfMod; auto).
+    assert (WfConcat2: forall ty, WfConcat ty m2 m1 ) by (intros; specialize (HWfMod ty); inv HWfMod; auto).
+    inv hwfmod2.
     pose proof (@split_Substeps1 (getFlat m1) (getFlat m2) HDisjRegs HDisjRules HDisjMeths WfBaseMod1 WfBaseMod2 _ _  ND_Regs1 ND_Regs2 H);dest.
     assert (Substeps (BaseMod (getAllRegisters m1) (getAllRules m1) (getAllMethods m1)) x (ModuleFilterLabels (getFlat m1) l) /\
             MatchingExecCalls_Base (ModuleFilterLabels (getFlat m1) l) (getFlat m1) /\
@@ -3256,13 +3273,13 @@ Proof.
   intros;unfold WeakEquality; split;[apply PermutationWI|apply PermutationWI;apply Permutation_sym];assumption.
 Qed.
 
-Lemma substitute_Step m o l (HWfMod: WfMod m):
+Lemma substitute_Step m o l (HWfMod: forall ty, WfMod ty m):
   Step (flatten m) o l ->
   exists l',
     Permutation l l' /\
     Step m o l'.
 Proof.
-  rewrite StepSubstitute_flatten in *; auto.
+  rewrite (@StepSubstitute_flatten (fun _ => unit)) in *; auto.
   apply substitute_Step'; auto.
 Qed.
 
@@ -3296,7 +3313,7 @@ Qed.
 
 Section TraceSubstitute.
   Variable m: Mod.
-  Variable WfMod_m: WfMod m.
+  Variable WfMod_m: forall ty, WfMod ty m.
 
   Lemma Trace_flatten_same1: forall o l,  Trace m o l -> Trace (flatten m) o l.
   Proof.
@@ -3305,7 +3322,7 @@ Section TraceSubstitute.
       unfold flatten.
       rewrite createHide_Regs.
       auto.
-    - apply Step_substitute in HStep; auto.
+    - apply (@Step_substitute type) in HStep; auto.
       econstructor 2; eauto.
   Qed.
 
@@ -3358,7 +3375,7 @@ Proof.
     repeat split; tauto.
 Qed.
 
-Lemma WfMod_createHide l: forall m, WfMod (createHide m l) <-> (SubList l (map fst (getMethods m)) /\ WfMod (Base m)).
+Lemma WfMod_createHide l: forall ty m, WfMod ty (createHide m l) <-> (SubList l (map fst (getMethods m)) /\ WfMod ty (Base m)).
 Proof.
   split.
   - induction l; simpl; intros; split; unfold SubList; simpl; intros; try tauto.
@@ -3371,14 +3388,14 @@ Proof.
     + apply IHl; intros; split;auto.
 Qed.
 
-Lemma WfActionT_flatten m k :
-  forall (a : ActionT type k),
+Lemma WfActionT_flatten ty m k :
+  forall (a : ActionT ty k),
     WfActionT m a <-> WfActionT (getFlat (Base m)) a.
 Proof.
   split; induction 1; econstructor; eauto.
 Qed.
 
-Lemma flatten_WfMod m: WfMod m -> WfMod (flatten m).
+Lemma flatten_WfMod ty m: WfMod ty m -> WfMod ty (flatten m).
 Proof.
   unfold flatten.
   induction 1; simpl; auto; intros.
@@ -3655,15 +3672,21 @@ Section ModularSubstition.
                                  (In x (map fst (getAllMethods b')) /\
                                   ~ In x (getHidden b')).
 
-  Variable wfAConcatB: WfMod (ConcatMod a b).
-  Variable wfA'ConcatB': WfMod (ConcatMod a' b').
+  Variable wfAConcatB: forall ty, WfMod ty (ConcatMod a b).
+  Variable wfA'ConcatB': forall ty, WfMod ty (ConcatMod a' b').
 
   Lemma ModularSubstition: TraceInclusion a a' ->
                            TraceInclusion b b' ->
                            TraceInclusion (ConcatMod a b) (ConcatMod a' b').
   Proof.
-    inv wfAConcatB.
-    inv wfA'ConcatB'.
+    assert (WfConcat1: forall ty, WfConcat ty a b) by (intros; specialize (wfAConcatB ty); inv wfAConcatB; auto).
+    assert (WfConcat2: forall ty, WfConcat ty b a) by (intros; specialize (wfAConcatB ty); inv wfAConcatB; auto).
+    assert (WfConcat0: forall ty, WfConcat ty a' b') by (intros; specialize (wfA'ConcatB' ty); inv wfA'ConcatB'; auto).
+    assert (WfConcat3: forall ty, WfConcat ty b' a') by (intros; specialize (wfA'ConcatB' ty); inv wfA'ConcatB'; auto).
+    pose proof (wfAConcatB (fun _ => unit)) as wfAConcatB_dup.
+    pose proof (wfA'ConcatB' (fun _ => unit)) as wfA'ConcatB'_dup.
+    inv wfAConcatB_dup.
+    inv wfA'ConcatB'_dup.
     unfold TraceInclusion, WeakInclusion,getListFullLabel_diff in *; intros.
     pose proof (SplitTrace HDisjRegs HDisjRules HDisjMeths H1); dest.
     specialize (@H _ _ H2).
@@ -3804,11 +3827,10 @@ Section ModularSubstition.
         rewrite H17. rewrite map_app, in_app_iff in *; setoid_rewrite in_app_iff.
         clear - H19 H18 H14.
         firstorder fail.
-Qed.
+  Qed.
 
 End ModularSubstition.
 
-Require Import Coq.Program.Equality.
 Section Fold.
   Variable k: Kind.
 
